Document Fuzz
Signed-off-by: zeramorphic <zeramorphic@proton.me>

ConNF/Fuzz/Construction.lean
@@ -1,13 +1,25 @@
 import ConNF.Fuzz.Hypotheses
 
 /-!
-# f-maps
+# Constructing the `fuzz` map
 
-Consider a code `(β, γ, G)`. We are interested in the alternative extensions of this object at
-different proper type indices `δ : Λ`. We will define the function `A_δ` which will map the code
-`(β, γ, G)` to a new code `(α, δ, D)`. The elements of `D` are produced by the so-called f-maps.
-In particular, elements of `D` are of the form `typed_near_litter M` where `M` is a near-litter to
-some litter `N`, which in turn is given by an f-map.
+In tangled type theory, a given model element has extensions at each level below it.
+We have a "preferred" extension, and must find a way to compute the other extensions from that
+information. In order to do this, we need to be able to convert arbitrary model elements into
+"junk" at other levels, which can then be clearly interpreted as a "non-preferred" extension.
+
+The `fuzz` maps perform this task. They are parametrised by a pair of type indices, representing
+the source type level and target type level. At each pair of levels, the `fuzz` map is an injection
+from tangles to litters. An arbitrary litter can only be the image of a `fuzz` map defined at a
+single pair of type levels.
+
+Treating the output of a `fuzz` map as a typed near-litter, its position is always greater than
+the position of the input to the function. This ensures a well-foundedness condition that we use
+in many places later.
+
+## Main declarations
+
+* `ConNF.fuzz`: Converts a tangle into a "junk" litter.
 -/
 
 open Cardinal Function Set WithBot
@@ -21,16 +33,15 @@ namespace ConNF
 section ChooseWf
 
 /-!
-We construct the f-maps by first defining the auxiliary function `choose_wf`.
+We construct the `fuzz` map by first defining the auxiliary function `chooseWf`.
 
 Suppose we wish to construct a function `f : α → β` with the constraint that for each `α`,
 there is a predefined set of "denied" `β` values that it cannot take. Under some restrictions
-based on the cardinalities of the denied set, we can construct such a function.
-We can in addition require that `f` be injective if `α` has a well-order, which we will assume here.
+based on the cardinalities of the denied set, we can construct such a function. We can in addition
+require that `f` be injective if `α` has a well-order, which we will assume here.
 
-The f-maps that we will construct indeed satisfy these conditions.
+The `fuzz` map that we will construct indeed satisfies these conditions.
 -/
-
 
 variable {α β : Type u} {r : α → α → Prop}
 
@@ -93,70 +104,68 @@ theorem chooseWf_injective [inst : IsWellOrder α r] {deny : α → Set β}
 end ChooseWf
 
 /-!
-We construct the f-maps by constructing a set of image values to deny, and then choosing
-arbitrarily from the remaining set. This uses the `choose_wf` results.
+We construct the `fuzz` maps by constructing a set of image values to deny, and then choosing
+arbitrarily from the remaining set. This uses the `chooseWf` results.
+
 The majority of this section is spent proving that the set of values to deny isn't "too large",
 such that we could run out of available values for the function.
 -/
-
 
 variable [Params.{u}] {β : TypeIndex} {γ : Λ} [TangleData β] [PositionFunction β]
   [BasePositions] [TangleData γ] [PositionFunction γ] [TypedObjects γ] (hβγ : β ≠ γ)
 
 /-- The requirements to be satisfied by the f-maps.
-If `fuzz_condition` applied to a litter indexed by `i` is true,
-then `i` is *not* a valid output to `fuzz x`. -/
-inductive FuzzCondition (x : Tangle β) (i : μ) : Prop
-  | any (N : Set Atom) (hN : IsNearLitter ⟨i, β, γ, hβγ⟩ N) :
-    position (typedNearLitter ⟨⟨i, β, γ, hβγ⟩, N, hN⟩ : Tangle γ) ≤ position x → FuzzCondition x i
+If `FuzzCondition` applied to a litter indexed by `ν` is true,
+then `ν` is *not* a valid output to `fuzz _ t`. -/
+inductive FuzzCondition (x : Tangle β) (ν : μ) : Prop
+  | any (N : Set Atom) (hN : IsNearLitter ⟨ν, β, γ, hβγ⟩ N) :
+    position (typedNearLitter ⟨⟨ν, β, γ, hβγ⟩, N, hN⟩ : Tangle γ) ≤ position x → FuzzCondition x ν
   | bot (a : Atom) :
-      β = ⊥ →   -- this condition should only trigger for type `-1`
-      HEq a x → -- using `heq` instead of induction on `β` or the instance deals with many annoyances
-      position (typedNearLitter (Litter.toNearLitter ⟨i, ⊥, γ, bot_ne_coe⟩) : Tangle γ) ≤
+      β = ⊥ →   -- this condition should only trigger for type `⊥`
+      HEq a x → -- using `HEq` instead of induction on `β` or the instance deals with some problems
+      position (typedNearLitter (Litter.toNearLitter ⟨ν, ⊥, γ, bot_ne_coe⟩) : Tangle γ) ≤
         typedAtomPosition a →
-      FuzzCondition x i
+      FuzzCondition x ν
 
 instance : IsWellOrder (Tangle β) (InvImage (· < ·) position) := by
   refine' { .. }
-  · intro x y
-    have := lt_trichotomy (position x) (position y)
+  · intro t₁ t₂
+    have := lt_trichotomy (position t₁) (position t₂)
     rw [EmbeddingLike.apply_eq_iff_eq] at this
     exact this
-  · intro x y z
+  · intro t₁ t₂ t₃
     exact lt_trans
   · exact InvImage.wf _ μwo.wf
 
 variable (γ)
 
-theorem mk_invImage_lt (x : Tangle β) : #{ y // InvImage (· < ·) position y x } < #μ := by
-  refine lt_of_le_of_lt ?_ (show #{ y // y < position x } < #μ from card_Iio_lt _)
+theorem mk_invImage_lt (t : Tangle β) : #{ y // InvImage (· < ·) position y t } < #μ := by
+  refine lt_of_le_of_lt ?_ (show #{ ν // ν < position t } < #μ from card_Iio_lt _)
   refine ⟨⟨fun y => ⟨_, y.prop⟩, ?_⟩⟩
   intro y₁ y₂ h
   simp only [Subtype.mk.injEq, EmbeddingLike.apply_eq_iff_eq, Subtype.coe_inj] at h
   exact h
 
-theorem mk_invImage_le (x : Tangle β) : #{ y : Tangle γ // position y ≤ position x } < #μ := by
-  refine lt_of_le_of_lt ?_ (show #{ y // y ≤ position x } < #μ from card_Iic_lt _)
-  refine ⟨⟨fun y => ⟨_, y.prop⟩, ?_⟩⟩
+theorem mk_invImage_le (t : Tangle β) : #{ t' : Tangle γ // position t' ≤ position t } < #μ := by
+  refine lt_of_le_of_lt ?_ (show #{ ν // ν ≤ position t } < #μ from card_Iic_lt _)
+  refine ⟨⟨fun t' => ⟨_, t'.prop⟩, ?_⟩⟩
   intro y₁ y₂ h
   simp only [Subtype.mk.injEq, EmbeddingLike.apply_eq_iff_eq, Subtype.coe_inj] at h
   exact h
 
 variable {γ}
 
-theorem mk_fuzz_deny (hβγ : β ≠ γ) (x : Tangle β) :
-    #{ y // InvImage (· < ·) position y x } + #{ i // FuzzCondition hβγ x i } < #μ := by
-  have h₁ := mk_invImage_lt x
-  suffices h₂ : #{ i // FuzzCondition hβγ x i } < #μ
+theorem mk_fuzz_deny (hβγ : β ≠ γ) (t : Tangle β) :
+    #{ t' // InvImage (· < ·) position t' t } + #{ ν // FuzzCondition hβγ t ν } < #μ := by
+  have h₁ := mk_invImage_lt t
+  suffices h₂ : #{ ν // FuzzCondition hβγ t ν } < #μ
   · exact add_lt_of_lt μ_isStrongLimit.isLimit.aleph0_le h₁ h₂
-  have : ∀ i, FuzzCondition hβγ x i →
-    (∃ (N : Set Atom) (hN : IsNearLitter ⟨i, β, γ, hβγ⟩ N),
-        position (typedNearLitter ⟨_, N, hN⟩ : Tangle γ) ≤ position x) ∨
-      β = ⊥ ∧
-        ∃ a : Atom,
-          HEq a x ∧
-            position (typedNearLitter (Litter.toNearLitter ⟨i, β, γ, hβγ⟩) : Tangle γ) ≤
-              typedAtomPosition a
+  have : ∀ ν, FuzzCondition hβγ t ν →
+    (∃ (N : Set Atom) (hN : IsNearLitter ⟨ν, β, γ, hβγ⟩ N),
+        position (typedNearLitter ⟨_, N, hN⟩ : Tangle γ) ≤ position t) ∨
+    (β = ⊥ ∧ ∃ a : Atom, HEq a t ∧
+    position (typedNearLitter (Litter.toNearLitter ⟨ν, β, γ, hβγ⟩) : Tangle γ) ≤
+      typedAtomPosition a)
   · intro i hi
     obtain ⟨N, hN₁, hN₂⟩ | ⟨a, h₁, h₂, h₃⟩ := hi
     · left; exact ⟨N, hN₁, hN₂⟩
@@ -164,19 +173,19 @@ theorem mk_fuzz_deny (hβγ : β ≠ γ) (x : Tangle β) :
   refine lt_of_le_of_lt (mk_subtype_mono this) ?_
   refine lt_of_le_of_lt (mk_union_le _ _) ?_
   refine add_lt_of_lt μ_isStrongLimit.isLimit.aleph0_le ?_ ?_
-  · refine lt_of_le_of_lt ?_ (mk_invImage_le γ x)
+  · refine lt_of_le_of_lt ?_ (mk_invImage_le γ t)
     refine ⟨⟨fun i => ⟨_, i.prop.choose_spec.choose_spec⟩, ?_⟩⟩
     intro i j h
     simp only [Subtype.mk.injEq, EmbeddingLike.apply_eq_iff_eq] at h
     apply_fun Sigma.fst at h
     simp only [Litter.mk.injEq, Subtype.coe_inj, and_self, and_true] at h
     exact h
-  · by_cases β = ⊥ ∧ ∃ a : Atom, HEq a x
+  · by_cases β = ⊥ ∧ ∃ a : Atom, HEq a t
     · obtain ⟨_, a, hax⟩ := h
       refine lt_of_le_of_lt ?_ (card_Iic_lt (typedAtomPosition a))
       refine ⟨⟨fun i => ⟨position (typedNearLitter
         (Litter.toNearLitter ⟨i, β, γ, hβγ⟩) : Tangle γ), ?_⟩, ?_⟩⟩
-      · obtain ⟨i, _, b, hb, _⟩ := i
+      · obtain ⟨ν, _, b, hb, _⟩ := i
         rw [eq_of_heq (hax.trans hb.symm)]
         assumption
       · intro i j h
@@ -190,51 +199,67 @@ theorem mk_fuzz_deny (hβγ : β ≠ γ) (x : Tangle β) :
       exact h ⟨hb, a, ha⟩
 
 /-!
-We're done with proving technical results, now we can define the f-maps.
+We're done with proving technical results, now we can define the `fuzz` maps.
 -/
 
-/-- The f-maps. -/
-noncomputable def fuzz (x : Tangle β) : Litter :=
-  ⟨chooseWf (FuzzCondition hβγ) (mk_fuzz_deny hβγ) x, β, γ, hβγ⟩
+/--
+The `fuzz` map for a particular pair of type indices.
+
+In tangled type theory, a given model element has extensions at each level below it.
+We have a "preferred" extension, and must find a way to compute the other extensions from that
+information. In order to do this, we need to be able to convert arbitrary model elements into
+"junk" at other levels, which can then be clearly interpreted as a "non-preferred" extension.
+
+The `fuzz` maps perform this task. They are parametrised by a pair of type indices, representing
+the source type level and target type level. At each pair of levels, the `fuzz` map is an injection
+from tangles to litters. An arbitrary litter can only be the image of a `fuzz` map defined at a
+single pair of type levels.
+
+Treating the output of a `fuzz` map as a typed near-litter, its position is always greater than
+the position of the input to the function. This ensures a well-foundedness condition that we use
+in many places later.
+-/
+noncomputable def fuzz (t : Tangle β) : Litter :=
+  ⟨chooseWf (FuzzCondition hβγ) (mk_fuzz_deny hβγ) t, β, γ, hβγ⟩
 
 @[simp]
-theorem fuzz_β (x : Tangle β) : (fuzz hβγ x).β = β :=
+theorem fuzz_β (t : Tangle β) : (fuzz hβγ t).β = β :=
   rfl
 
 @[simp]
-theorem fuzz_γ (x : Tangle β) : (fuzz hβγ x).γ = γ :=
+theorem fuzz_γ (t : Tangle β) : (fuzz hβγ t).γ = γ :=
   rfl
 
 theorem fuzz_injective : Injective (fuzz hβγ) := by
-  intro x y h
+  intro t₁ t₂ h
   simp only [fuzz, Litter.mk.injEq, chooseWf_injective.eq_iff, and_self, and_true] at h
   exact h
 
-theorem fuzz_not_mem_deny (x : Tangle β) : (fuzz hβγ x).ν ∉ {i | FuzzCondition hβγ x i} :=
-  chooseWf_not_mem_deny x
+theorem fuzz_not_mem_deny (t : Tangle β) : (fuzz hβγ t).ν ∉ {ν | FuzzCondition hβγ t ν} :=
+  chooseWf_not_mem_deny t
 
-theorem fuzz_position' (x : Tangle β) (N : Set Atom) (h : IsNearLitter (fuzz hβγ x) N) :
-    position x < position (typedNearLitter ⟨fuzz hβγ x, N, h⟩ : Tangle γ) := by
-  have h' := fuzz_not_mem_deny hβγ x
+theorem fuzz_position' (t : Tangle β) (N : Set Atom) (h : IsNearLitter (fuzz hβγ t) N) :
+    position t < position (typedNearLitter ⟨fuzz hβγ t, N, h⟩ : Tangle γ) := by
+  have h' := fuzz_not_mem_deny hβγ t
   contrapose! h'
   -- Generalise the instances.
   revert β
   intro β
   induction β using WithBot.recBotCoe <;>
-  · intros _ _ hβγ x h h'
+  · intros _ _ hβγ t h h'
     exact FuzzCondition.any _ h h'
 
-theorem fuzz_position (x : Tangle β) (N : NearLitter) (h : N.1 = fuzz hβγ x) :
-    position x < position (typedNearLitter N : Tangle γ) := by
-  have := fuzz_position' hβγ x N ((NearLitter.isNearLitter _ _).mpr h)
+theorem fuzz_position (t : Tangle β) (N : NearLitter) (h : N.1 = fuzz hβγ t) :
+    position t < position (typedNearLitter N : Tangle γ) := by
+  have := fuzz_position' hβγ t N ((NearLitter.isNearLitter _ _).mpr h)
   exact lt_of_lt_of_eq this (congr_arg _ (congr_arg _ (NearLitter.ext rfl)))
 
-theorem typedAtomPosition_lt_fuzz (x : Tangle ⊥) :
-  typedAtomPosition x <
+theorem typedAtomPosition_lt_fuzz (t : Tangle ⊥) :
+  typedAtomPosition t <
     position
-      (typedNearLitter (fuzz (bot_ne_coe : (⊥ : TypeIndex) ≠ γ) x).toNearLitter : Tangle γ) := by
-  have := fuzz_not_mem_deny (bot_ne_coe : (⊥ : TypeIndex) ≠ γ) x
+      (typedNearLitter (fuzz (bot_ne_coe : (⊥ : TypeIndex) ≠ γ) t).toNearLitter : Tangle γ) := by
+  have := fuzz_not_mem_deny (bot_ne_coe : (⊥ : TypeIndex) ≠ γ) t
   contrapose! this
-  exact FuzzCondition.bot x rfl HEq.rfl this
+  exact FuzzCondition.bot t rfl HEq.rfl this
 
 end ConNF
